Bdd/Prime.lean
@@ -14,8 +14,8 @@ lemma prime_edge_iff {B : Bdd n m} {x y : Pointer m} : Edge B.heap x y ↔ Edge 
   constructor
   · intro e
     cases e with
-    | low  _ => left;  simpa [prime, prime_heap, prime_node]
-    | high _ => right; simpa [prime, prime_heap, prime_node]
+    | low  _ => left;  simpa [prime, prime_heap]
+    | high _ => right; simpa [prime, prime_heap]
   · intro e
     cases e with
     | low  _ => left;  simp_all [prime, prime_heap, prime_node]; assumption
@@ -372,5 +372,461 @@ lemma oprime_reduced {O : OBdd n m} : O.Reduced → (oprime p O).Reduced := by
   constructor
   · exact prime_preserves_noRedundancy r1
   · rintro _ _ sim; exact r2 (oprime_preserves_similarRP sim)
+
+def unprime_node (p : Fin n) : Node n m → Node (n - p) m
+  | ⟨var, low, high⟩ => ⟨⟨var.1 - p.1, by omega⟩, low, high⟩
+
+def unprime_heap (p : Fin n) : Vector (Node n m) m → Vector (Node (n - p) m) m := Vector.map (unprime_node p)
+
+def unprime (p : Fin n) : Bdd n m → Bdd (n - p) m
+  | ⟨heap, root⟩ => ⟨unprime_heap p heap, root⟩
+
+lemma unprime_edge_iff {B : Bdd n m} {x y : Pointer m} : Edge B.heap x y ↔ Edge (unprime p B).heap x y := by
+  constructor
+  · intro e
+    cases e with
+    | low  _ => left;  simpa [unprime, unprime_heap]
+    | high _ => right; simpa [unprime, unprime_heap]
+  · intro e
+    cases e with
+    | low  _ => left;  simp_all [unprime, unprime_heap]; assumption
+    | high _ => right; simp_all [unprime, unprime_heap]; assumption
+
+lemma unprime_reachable_iff {B : Bdd n m} : Pointer.Reachable B.heap B.root x ↔ Pointer.Reachable (unprime p B).heap (unprime p B).root x := by
+  constructor
+  · intro r
+    induction r with
+    | refl => left
+    | tail _ e ih =>
+      right
+      · exact ih
+      · exact (unprime_edge_iff.mp e)
+  · intro r
+    induction r with
+    | refl => left
+    | tail _ e ih =>
+      right
+      · exact ih
+      · exact (unprime_edge_iff.mpr e)
+
+lemma unprime_mayPrecede {B : Bdd n m} {x y : Pointer m} {p : Fin n} : p ≤ x.toVar B.heap → Pointer.MayPrecede B.heap x y → Pointer.MayPrecede (unprime p B).heap x y := by
+  intro hp h
+  cases x with
+  | terminal _ => absurd h; exact Pointer.not_terminal_MayPrecede
+  | node _ =>
+    cases y with
+    | terminal _ => apply Pointer.MayPrecede_node_terminal
+    | node _ =>
+      simp only [Pointer.MayPrecede, unprime, unprime_heap, Pointer.toVar] at h
+      simp only [Nat.succ_eq_add_one, Fin.getElem_fin, Fin.coe_eq_castSucc, Fin.castSucc_lt_castSucc_iff] at h
+      simp only [Pointer.MayPrecede, unprime, unprime_heap, Pointer.toVar]
+      simp only [Nat.succ_eq_add_one, Fin.getElem_fin, Vector.getElem_map, Fin.coe_eq_castSucc, Fin.castSucc_lt_castSucc_iff]
+      simp only [unprime_node]
+      simp only [Fin.eta, Fin.mk_lt_mk, add_lt_add_iff_right, Fin.val_fin_lt]
+      refine Nat.sub_lt_sub_right ?_ h
+      simp only [Nat.succ_eq_add_one, Fin.coe_eq_castSucc, Pointer.toVar_node_eq, Fin.getElem_fin, Fin.castSucc_le_castSucc_iff] at hp
+      exact hp
+
+lemma unprime_relevantMayPrecede {B : Bdd n m} {x y : Pointer m} {hx : Pointer.Reachable (unprime p B).heap (unprime p B).root x} {hy : Pointer.Reachable (unprime p B).heap (unprime p B).root y} :
+    p ≤ x.toVar B.heap → B.RelevantMayPrecede ⟨x, unprime_reachable_iff.mpr hx⟩ ⟨y, unprime_reachable_iff.mpr hy⟩ → (unprime p B).RelevantMayPrecede ⟨x, hx⟩ ⟨y, hy⟩ := unprime_mayPrecede
+
+lemma unprime_relevantEdge {B : Bdd n m} {x y : Pointer m} {hx : Pointer.Reachable (unprime p B).heap (unprime p B).root x} {hy : Pointer.Reachable (unprime p B).heap (unprime p B).root y} :
+    (unprime p B).RelevantEdge ⟨x, hx⟩ ⟨y, hy⟩ → B.RelevantEdge ⟨x, unprime_reachable_iff.mpr hx⟩ ⟨y, unprime_reachable_iff.mpr hy⟩ := by
+  intro h
+  simp_all only [Bdd.RelevantEdge, unprime, unprime_heap]
+  cases h with
+  | low _ =>
+    left
+    simp_all [unprime_node]
+    assumption
+  | high _ =>
+    right
+    simp_all [unprime_node]
+    assumption
+
+lemma unprime_preserves_ordered {B : Bdd n m} {p : Fin n} : p ≤ B.var → Bdd.Ordered B → Bdd.Ordered (unprime p B) := by
+  intro hp ho
+  rintro ⟨x, hx⟩ _ hxy
+  apply unprime_relevantMayPrecede
+  · simp only [Nat.succ_eq_add_one, Fin.coe_eq_castSucc, Bdd.var] at hp
+    simp only [Nat.succ_eq_add_one, Fin.coe_eq_castSucc]
+    trans Pointer.toVar B.heap B.root
+    exact hp
+    apply Pointer.mayPrecede_of_reachable ho (unprime_reachable_iff.mpr hx)
+  · apply ho
+    exact unprime_relevantEdge hxy
+
+def ounprime (p : Fin n) (O : OBdd n m) : p ≤ O.1.var → OBdd (n - p) m
+  | hp => ⟨unprime p O.1, unprime_preserves_ordered hp O.2⟩
+
+lemma ounprime_low {O : OBdd n m} {h : O.1.root = .node j} {p: Fin n} {hp : p ≤ O.1.var} :
+    (OBdd.low (ounprime p O hp) h) = ounprime p (O.low h) (by trans O.1.var; exact hp; apply le_of_lt OBdd.var_lt_low_var) := by
+  rcases O with ⟨B, o⟩
+  simp only [OBdd.low]
+  congr
+  simp only [ounprime, unprime, unprime_heap, Bdd.low_heap_eq_heap]
+  simp only at h
+  simp_rw [h]
+  simp only [Bdd.low]
+  congr 1
+  simp_all only [Fin.getElem_fin, Vector.getElem_map]
+  rfl
+
+lemma ounprime_high {O : OBdd n m} {h : O.1.root = .node j} {p: Fin n} {hp : p ≤ O.1.var} :
+    (OBdd.high (ounprime p O hp) h) = ounprime p (O.high h) (by trans O.1.var; exact hp; apply le_of_lt OBdd.var_lt_high_var) := by
+  rcases O with ⟨B, o⟩
+  simp only [OBdd.high]
+  congr
+  simp only [ounprime, unprime, unprime_heap, Bdd.high_heap_eq_heap]
+  simp only at h
+  simp_rw [h]
+  simp only [Bdd.high]
+  congr 1
+  simp_all only [Fin.getElem_fin, Vector.getElem_map]
+  rfl
+
+lemma bunprime_low {n m j} {B : Bdd n m} {o : Bdd.Ordered B} {h : B.root = .node j} {p: Fin n} {hp : p ≤ B.var} :
+    (OBdd.low ⟨unprime p B, unprime_preserves_ordered hp o⟩ h) =
+    ⟨unprime p (OBdd.low ⟨B, o⟩ h).1,
+     unprime_preserves_ordered
+      (by trans B.var; exact hp; apply le_of_lt; rw [show B.var = (⟨B, o⟩ : OBdd n m).1.var by rfl]; apply OBdd.var_lt_low_var)
+      (OBdd.low ⟨B, o⟩ h).2⟩ := by
+  simp only [OBdd.low]
+  congr
+  simp only [unprime, unprime_heap, Bdd.low_heap_eq_heap]
+  simp_rw [h]
+  simp only [Bdd.low]
+  congr 1
+  simp_all only [Fin.getElem_fin, Vector.getElem_map]
+  rfl
+
+lemma bunprime_high {n m j} {B : Bdd n m} {o : Bdd.Ordered B} {h : B.root = .node j} {p: Fin n} {hp : p ≤ B.var} :
+    (OBdd.high ⟨unprime p B, unprime_preserves_ordered hp o⟩ h) =
+    ⟨unprime p (OBdd.high ⟨B, o⟩ h).1,
+     unprime_preserves_ordered
+      (by trans B.var; exact hp; apply le_of_lt; rw [show B.var = (⟨B, o⟩ : OBdd n m).1.var by rfl]; apply OBdd.var_lt_high_var)
+      (OBdd.high ⟨B, o⟩ h).2⟩ := by
+  simp only [OBdd.high]
+  congr
+  simp only [unprime, unprime_heap, Bdd.high_heap_eq_heap]
+  simp_rw [h]
+  simp only [Bdd.high]
+  congr 1
+  simp_all only [Fin.getElem_fin, Vector.getElem_map]
+  rfl
+
+theorem ounprime_evaluate (O : OBdd n m) {p : Fin n} (hp : p ≤ O.1.var) {I : Vector Bool (n - p)} {J : Vector Bool p} : OBdd.evaluate (ounprime p O hp) I = O.evaluate (Vector.cast (by omega) (J ++ I)) := by
+  simp only [ounprime]
+  cases O_root_def : O.1.root with
+  | terminal _ =>
+    simp only [unprime]
+    rw [OBdd.evaluate_terminal' O_root_def]
+    simp_rw [O_root_def]
+    rw [OBdd.evaluate_terminal]
+    simp
+  | node j =>
+    rw [OBdd.evaluate_node'' O_root_def]
+    have that : (⟨(unprime p O.1), unprime_preserves_ordered hp O.2⟩ : OBdd _ _).1.root = Pointer.node j := O_root_def
+    rw [OBdd.evaluate_node'' that]
+    simp only
+    congr 1
+    · simp only [eq_iff_iff, Bool.coe_iff_coe]
+      simp only [unprime, unprime_heap, Fin.getElem_fin, Vector.getElem_map, unprime_node]
+      simp only [Fin.eta]
+      rw [Vector.getElem_cast]
+      rw [Vector.getElem_append]
+      split
+      next contra =>
+        absurd contra
+        simp only [Nat.succ_eq_add_one, Fin.coe_eq_castSucc, Bdd.var] at hp
+        rw [O_root_def] at hp
+        simp at hp
+        omega
+      next => rfl
+    · have := ounprime_evaluate (O.high O_root_def) (I := I) (J := J)
+      rw [← this]
+      rw [← ounprime_high (hp := hp)]
+      rfl
+    · have := ounprime_evaluate (O.low O_root_def) (I := I) (J := J)
+      rw [← this]
+      rw [← ounprime_low (hp := hp)]
+      rfl
+termination_by O
+
+def tunprime (p : Fin n) (T : DecisionTree n) : T.lowerBoundedBy p → DecisionTree (n - p) := fun r ↦
+  match T with
+  | .leaf b => .leaf b
+  | .branch i l h => .branch ⟨i.1 - p, by omega⟩ (tunprime p l (DecisionTree.lowerBoundedBy_low r)) (tunprime p h (DecisionTree.lowerBoundedBy_high r))
+
+lemma tunprime_injective : tunprime x T1 h1 = tunprime x T2 h2 → T1 = T2 := by
+  intro h
+  cases T1 with
+  | leaf _ =>
+    cases T2 with
+    | leaf _ => simp only [tunprime] at h; simp_all
+    | branch _ _ _ => contradiction
+  | branch v1 l1 r1 =>
+    cases T2 with
+    | leaf _ => contradiction
+    | branch v2 l2 r2 =>
+      simp only [tunprime] at h
+      injection h with a b c
+      rw [tunprime_injective b, tunprime_injective c]
+      simp_all only [Fin.mk.injEq, DecisionTree.branch.injEq, and_self, and_true]
+      have : x.1 ≤ v1.1 := by
+        cases h1 with
+        | node _ _ _ => assumption
+      have : x.1 ≤ v2.1 := by
+        cases h2 with
+        | node _ _ _ => assumption
+      omega
+
+lemma unprime_low {O : OBdd n m} {h : O.1.root = .node j} {p : Fin n} {hp : p ≤ O.1.var} :
+   (OBdd.low ⟨unprime p O.1, unprime_preserves_ordered hp O.2⟩ h) = ⟨unprime p (O.low h).1, unprime_preserves_ordered (by trans O.1.var; exact hp; apply le_of_lt; apply OBdd.var_lt_low_var) (O.low h).2⟩ := by
+  simp only [OBdd.low]
+  congr
+  simp only [unprime, unprime_heap, Bdd.low_heap_eq_heap]
+  simp_rw [h]
+  simp only [Bdd.low]
+  congr 1
+  simp_all only [Fin.getElem_fin, Vector.getElem_map]
+  rfl
+
+lemma unprime_high {O : OBdd n m} {h : O.1.root = .node j} {p : Fin n} {hp : p ≤ O.1.var} :
+   (OBdd.high ⟨unprime p O.1, unprime_preserves_ordered hp O.2⟩ h) = ⟨unprime p (O.high h).1, unprime_preserves_ordered (by trans O.1.var; exact hp; apply le_of_lt; apply OBdd.var_lt_high_var) (O.high h).2⟩ := by
+  simp only [OBdd.high]
+  congr
+  simp only [unprime, unprime_heap, Bdd.high_heap_eq_heap]
+  simp_rw [h]
+  simp only [Bdd.high]
+  congr 1
+  simp_all only [Fin.getElem_fin, Vector.getElem_map]
+  rfl
+
+lemma unprime_toTree_tunprime' {O : OBdd n m} {p : Fin n} {hp : p ≤ O.1.var} :
+    OBdd.toTree ⟨unprime p O.1, unprime_preserves_ordered hp O.2⟩ = tunprime p (OBdd.toTree O) (OBdd.toTree_lowerBoundedBy_var hp) := by
+  cases O_root_def : O.1.root with
+  | terminal _ =>
+    simp only [unprime]
+    simp_rw [OBdd.toTree_terminal' O_root_def]
+    simp_rw [O_root_def]
+    rw [OBdd.toTree_terminal]
+    simp [tunprime]
+  | node _ =>
+    simp_rw [OBdd.toTree_node O_root_def]
+    rw [OBdd.toTree_node (by trans O.1.root; rfl; exact O_root_def)]
+    simp only [Fin.getElem_fin]
+    congr 1
+    · simp only [unprime, unprime_heap, Vector.getElem_map, unprime_node, Fin.eta, Bdd.Ordered.eq_1, Fin.mk.injEq, Nat.add_right_cancel_iff]
+      rfl
+    · have := unprime_toTree_tunprime' (O := (O.low O_root_def)) (p := p) (hp := (by trans O.1.var; exact hp; apply le_of_lt OBdd.var_lt_low_var))
+      rw [← unprime_low (hp := hp)] at this
+      exact this
+    · have := unprime_toTree_tunprime' (O := (O.high O_root_def)) (p := p) (hp := (by trans O.1.var; exact hp; apply le_of_lt OBdd.var_lt_high_var))
+      rw [← unprime_high (hp := hp)] at this
+      exact this
+termination_by O
+
+lemma unprime_toTree_tunprime {B : Bdd n m} {o : B.Ordered} {p : Fin n} {hp : p ≤ B.var} :
+    OBdd.toTree ⟨unprime p B, unprime_preserves_ordered hp o⟩ = tunprime p (OBdd.toTree ⟨B, o⟩) (OBdd.toTree_lowerBoundedBy_var hp) := by
+  let O : OBdd n m := ⟨B, o⟩
+  have : B = O.1 := rfl
+  simp_rw [this]
+  exact unprime_toTree_tunprime' (hp := hp)
+
+lemma unprime_preserves_noRedundancy {B : Bdd n m} : B.NoRedundancy → (unprime p B).NoRedundancy := by
+  rintro hnr ⟨p, hp⟩ contra
+  simp only at contra
+  cases p_def : p with
+  | terminal _ =>
+    cases contra with
+    | red _ => contradiction
+  | node j =>
+    rw [p_def] at contra
+    cases contra with
+    | red red =>
+      simp only [unprime, unprime_heap, Fin.getElem_fin, unprime_node] at red
+      apply hnr ⟨p, unprime_reachable_iff.mpr hp⟩
+      simp_rw [p_def]
+      constructor
+      simp_all only [Vector.getElem_map, Fin.getElem_fin]
+      simp only [unprime, unprime_heap, Fin.getElem_fin, unprime_node] at red
+      exact red
+
+lemma ounprime_preserves_similarRP {O : OBdd n m} {p q : Pointer m} {hx}
+    {hp : Pointer.Reachable (ounprime x O hx).1.heap (ounprime x O hx).1.root p} {hq : Pointer.Reachable (ounprime x O hx).1.heap (ounprime x O hx).1.root q} :
+    (ounprime x O hx).SimilarRP ⟨p, hp⟩ ⟨q, hq⟩ → O.SimilarRP ⟨p, unprime_reachable_iff.mpr hp⟩ ⟨q, unprime_reachable_iff.mpr hq⟩ := by
+  intro sim
+  simp only [OBdd.SimilarRP, OBdd.Similar, OBdd.HSimilar] at sim
+  simp only [OBdd.SimilarRP, OBdd.Similar, OBdd.HSimilar]
+  cases p with
+  | terminal _ =>
+    cases q with
+    | terminal _ => simp_all
+    | node _ =>
+      simp only [OBdd.toTree_terminal] at sim
+      rw [OBdd.toTree_node rfl] at sim
+      contradiction
+  | node j =>
+    cases q with
+    | terminal _ =>
+      simp only [OBdd.toTree_terminal] at sim
+      rw [OBdd.toTree_node rfl] at sim
+      contradiction
+    | node i =>
+      conv at sim =>
+        lhs
+        rw [OBdd.toTree_node rfl]
+      conv at sim =>
+        rhs
+        rw [OBdd.toTree_node rfl]
+      injection sim with ha hb hc
+      simp only [Fin.getElem_fin] at ha
+      simp only [ounprime, unprime, unprime_heap, Vector.getElem_map, unprime_node, Fin.eta, Fin.mk.injEq, Nat.add_right_cancel_iff] at ha
+      conv =>
+        lhs
+        rw [OBdd.toTree_node rfl]
+      conv =>
+        rhs
+        rw [OBdd.toTree_node rfl]
+      have this : x ≤ O.1.heap[j].var := by
+        apply Fin.le_iff_val_le_val.mpr
+        trans O.1.var.1
+        · simp only [Nat.succ_eq_add_one, Fin.coe_eq_castSucc, Bdd.var] at hx
+          simp only [Nat.succ_eq_add_one, Bdd.var]
+          exact hx
+        · have := Pointer.mayPrecede_of_reachable O.2 (unprime_reachable_iff.mpr hp)
+          simp only [Nat.succ_eq_add_one, Pointer.toVar_node_eq, Fin.getElem_fin, Fin.coe_eq_castSucc] at this
+          simp only [Nat.succ_eq_add_one, Bdd.var, Fin.getElem_fin, ge_iff_le]
+          exact this
+      have that : x ≤ O.1.heap[i].var := by
+        apply Fin.le_iff_val_le_val.mpr
+        trans O.1.var.1
+        · simp only [Nat.succ_eq_add_one, Fin.coe_eq_castSucc, Bdd.var] at hx
+          simp only [Nat.succ_eq_add_one, Bdd.var]
+          exact hx
+        · have := Pointer.mayPrecede_of_reachable O.2 (unprime_reachable_iff.mpr hq)
+          simp only [Nat.succ_eq_add_one, Pointer.toVar_node_eq, Fin.getElem_fin, Fin.coe_eq_castSucc] at this
+          simp only [Nat.succ_eq_add_one, Bdd.var, Fin.getElem_fin, ge_iff_le]
+          exact this
+      congr 1
+      · simp only
+        simp_all only [Fin.getElem_fin]
+        suffices s : O.1.heap[j.1].var - x.1 = O.1.heap[i.1].var - x.1 by omega
+        exact ha
+      · simp only [ounprime] at hb
+        simp only [unprime] at hb
+        simp_rw [← unprime.eq_1] at hb
+        conv at hb =>
+          lhs
+          rw [bunprime_low (h := rfl) (hp := (by simp; exact this)) (o := Bdd.ordered_of_reachable (unprime_reachable_iff.mpr hp))]
+        conv at hb =>
+          rhs
+          rw [bunprime_low (h := rfl) (hp := (by simp; exact that)) (o := Bdd.ordered_of_reachable (unprime_reachable_iff.mpr hq))]
+        simp only [OBdd.low] at hb
+        simp only [OBdd.low]
+        have this : x ≤ Pointer.toVar O.1.heap O.1.heap[j].low := by
+          apply Fin.le_iff_val_le_val.mpr
+          trans O.1.var.1
+          · simp only [Nat.succ_eq_add_one, Fin.coe_eq_castSucc, Bdd.var] at hx
+            simp only [Nat.succ_eq_add_one, Bdd.var]
+            simp_all
+            exact hx
+          · have := Pointer.mayPrecede_of_reachable O.2 (unprime_reachable_iff.mpr hp)
+            simp only [Nat.succ_eq_add_one, Pointer.toVar_node_eq, Fin.getElem_fin, Fin.coe_eq_castSucc] at this
+            simp only [Nat.succ_eq_add_one, Bdd.var, Fin.getElem_fin, ge_iff_le]
+            simp_all
+            apply Pointer.mayPrecede_of_reachable O.2
+            trans .node j
+            exact (unprime_reachable_iff.mpr hp)
+            apply Bdd.reachable_of_edge
+            left
+            rfl
+        have that : x ≤ Pointer.toVar O.1.heap O.1.heap[i].low := by
+          apply Fin.le_iff_val_le_val.mpr
+          trans O.1.var.1
+          · simp only [Nat.succ_eq_add_one, Fin.coe_eq_castSucc, Bdd.var] at hx
+            simp only [Nat.succ_eq_add_one, Bdd.var]
+            simp_all
+            exact hx
+          · have := Pointer.mayPrecede_of_reachable O.2 (unprime_reachable_iff.mpr hq)
+            simp only [Nat.succ_eq_add_one, Pointer.toVar_node_eq, Fin.getElem_fin, Fin.coe_eq_castSucc] at this
+            simp only [Nat.succ_eq_add_one, Bdd.var, Fin.getElem_fin, ge_iff_le]
+            simp_all
+            apply Pointer.mayPrecede_of_reachable O.2
+            trans .node i
+            exact (unprime_reachable_iff.mpr hq)
+            apply Bdd.reachable_of_edge
+            left
+            rfl
+        conv at hb =>
+          lhs
+          rw [unprime_toTree_tunprime (o := (by apply Bdd.low_ordered; exact Bdd.ordered_of_reachable (unprime_reachable_iff.mpr hp)))
+                                      (hp := (by exact this))]
+        conv at hb =>
+          rhs
+          rw [unprime_toTree_tunprime (o := (by apply Bdd.low_ordered; exact Bdd.ordered_of_reachable (unprime_reachable_iff.mpr hq)))
+                                      (hp := (by exact that))]
+        rw [tunprime_injective hb]
+      · simp only [ounprime] at hc
+        simp only [unprime] at hc
+        simp_rw [← unprime.eq_1] at hc
+        conv at hc =>
+          lhs
+          rw [bunprime_high (h := rfl) (hp := (by simp; exact this)) (o := Bdd.ordered_of_reachable (unprime_reachable_iff.mpr hp))]
+        conv at hc =>
+          rhs
+          rw [bunprime_high (h := rfl) (hp := (by simp; exact that)) (o := Bdd.ordered_of_reachable (unprime_reachable_iff.mpr hq))]
+        simp only [OBdd.high] at hc
+        simp only [OBdd.high]
+        have this : x ≤ Pointer.toVar O.1.heap O.1.heap[j].high := by
+          apply Fin.le_iff_val_le_val.mpr
+          trans O.1.var.1
+          · simp only [Nat.succ_eq_add_one, Fin.coe_eq_castSucc, Bdd.var] at hx
+            simp only [Nat.succ_eq_add_one, Bdd.var]
+            simp_all
+            exact hx
+          · have := Pointer.mayPrecede_of_reachable O.2 (unprime_reachable_iff.mpr hp)
+            simp only [Nat.succ_eq_add_one, Pointer.toVar_node_eq, Fin.getElem_fin, Fin.coe_eq_castSucc] at this
+            simp only [Nat.succ_eq_add_one, Bdd.var, Fin.getElem_fin, ge_iff_le]
+            simp_all
+            apply Pointer.mayPrecede_of_reachable O.2
+            trans .node j
+            exact (unprime_reachable_iff.mpr hp)
+            apply Bdd.reachable_of_edge
+            right
+            rfl
+        have that : x ≤ Pointer.toVar O.1.heap O.1.heap[i].high := by
+          apply Fin.le_iff_val_le_val.mpr
+          trans O.1.var.1
+          · simp only [Nat.succ_eq_add_one, Fin.coe_eq_castSucc, Bdd.var] at hx
+            simp only [Nat.succ_eq_add_one, Bdd.var]
+            simp_all
+            exact hx
+          · have := Pointer.mayPrecede_of_reachable O.2 (unprime_reachable_iff.mpr hq)
+            simp only [Nat.succ_eq_add_one, Pointer.toVar_node_eq, Fin.getElem_fin, Fin.coe_eq_castSucc] at this
+            simp only [Nat.succ_eq_add_one, Bdd.var, Fin.getElem_fin, ge_iff_le]
+            simp_all
+            apply Pointer.mayPrecede_of_reachable O.2
+            trans .node i
+            exact (unprime_reachable_iff.mpr hq)
+            apply Bdd.reachable_of_edge
+            right
+            rfl
+        conv at hc =>
+          lhs
+          rw [unprime_toTree_tunprime (o := (by apply Bdd.high_ordered; exact Bdd.ordered_of_reachable (unprime_reachable_iff.mpr hp)))
+                                      (hp := (by exact this))]
+        conv at hc =>
+          rhs
+          rw [unprime_toTree_tunprime (o := (by apply Bdd.high_ordered; exact Bdd.ordered_of_reachable (unprime_reachable_iff.mpr hq)))
+                                      (hp := (by exact that))]
+        rw [tunprime_injective hc]
+
+lemma ounprime_reduced {O : OBdd n m} {p : Fin n} {hp : p ≤ O.1.var} : O.Reduced → (ounprime p O hp).Reduced := by
+  rintro ⟨r1, r2⟩
+  constructor
+  · exact unprime_preserves_noRedundancy r1
+  · rintro _ _ sim; exact r2 (ounprime_preserves_similarRP sim)
 
 end Prime
